worked on proof of iter laws and that obs forms an iter morphism

theories/Dijkstra/IterRel.v
@@ -1,3 +1,4 @@
+From Coq Require Import Logic.Classical_Prop.
 From Paco Require Import paco.
 
 Section IterRel.
@@ -25,6 +26,43 @@ Section IterRel.
   Definition not_wf_from : A -> Prop :=
     paco1 not_wf_F bot1.
 
+  Inductive wf_from : A -> Prop :=
+    | base (a : A) : (forall a', ~ (r a a')) -> wf_from a
+    | step (a : A) : (forall a', r a a' -> wf_from a') -> wf_from a
+  .
+  Hint Constructors wf_from.
+  Lemma neg_wf_from_not_wf_from_l : forall (a : A),
+      ~(wf_from a) -> not_wf_from a.
+  Proof.
+    pcofix CIH. intros. pfold. destruct (classic (exists a', r a a' /\ ~ ( wf_from a') )).
+    - destruct H as [a' [Hr Hwf] ]. econstructor; eauto.
+    - assert (forall a', ~ r a a' \/ wf_from a').
+      {
+        intros.
+        destruct (classic (r a a')); auto. destruct (classic (wf_from a')); auto.
+        exfalso. apply H. exists a'. auto.
+      }
+      clear H.
+      exfalso. apply H0. clear H0. apply step. intros. destruct (H1 a'); auto.
+  Qed.
+
+  Lemma neg_wf_from_not_wf_from_r : forall (a : A),
+      not_wf_from a -> ~ (wf_from a).
+  Proof.
+    intros. intro Hcontra. punfold H.  inversion H. pclearbot. clear H. generalize dependent a'. 
+    induction Hcontra; intros.
+    - apply H in Hrel. auto.
+    - punfold Hcorec. inversion Hcorec. pclearbot. specialize (H0 a' Hrel a'0 Hrel0).
+      auto.
+  Qed.
+
+  Lemma neg_wf_from_not_wf_from : forall (a : A),
+      not_wf_from a <-> ~(wf_from a).
+  Proof.
+    split; try apply neg_wf_from_not_wf_from_r; try apply neg_wf_from_not_wf_from_l.
+  Qed.
+
+  
 End IterRel.
 
 
