theories/Dijkstra/PureITreeIter.v
@@ -124,6 +124,9 @@ Proof.
   cbn. intros. dest_dep g a. eapply Hfa; try apply H0. intros t Ht. inversion Ht; eauto.
 Qed.
 
+Definition iter_fix_n {A B : Type} (n : nat)  
+           (g :  A -> PureITreeSpec (A + B) ) (a : A) : PureITreeSpec B :=
+  exist _ (approx_iter_fix n g a) (iter_fix_monot_aux A B n g a).
 
 Lemma iter_fix_monot : forall A B (g :  A -> PureITreeSpec (A + B) ) (a : A),
                               monotonici B ( _iter_fix g a).
@@ -167,33 +170,84 @@ Proof.
   intros. rewrite H. reflexivity.
 Qed.
 
+Lemma observe_eutt_spin : forall E A (t : itree E A), t ≈ spin -> exists t0, observe t = TauF t0 /\ t0 ≈ spin.
+Proof.
+  intros. destruct (observe t) eqn : Heq; try discriminate.
+  - specialize (itree_eta t) as Heta. rewrite Heq in Heta. rewrite Heta in H. pinversion H. 
+    destruct (observe spin) eqn : ?Heq; try discriminate. admit.
+  - exists t0. split; auto. specialize (itree_eta t) as H0. rewrite Heq in H0. rewrite H0 in H.
+    rewrite tau_eutt in H. auto.
+  - specialize (itree_eta t) as Heta. rewrite Heq in Heta. rewrite Heta in H. exfalso. clear Heq Heta.
+    admit.
+Admitted.
+
 (*could use yannick or Li Yao's help on this one, should be true but has been problematic
   to prove*)
 Lemma not_wf_iter_spin : forall (A B : Type) (g : A -> itree Void (A + B) ) (a : A),
           not_wf_from A (fun a1 a2 => a1 =[ fun x => obs _ (g x) ]=> a2) a -> spin ≈ iter g a.
 Proof.
-  intros. generalize dependent a. pcofix CIH. intros. 
-  pfold. punfold H0.
-  - inversion H0. pclearbot. unfold spec_iter_arrow_rel in Hrel. cbn in Hrel. red in Hrel.
-    specialize (unfold_iter_ktree g a) as Hiter. apply strong_to_weak_bisim in Hiter as Hiter'.
-    rewrite Hrel in Hiter'. setoid_rewrite bind_ret in Hiter'. 
-    destruct (observe (@spin Void B)) eqn : Heq; try discriminate.
-    red. rewrite Heq. 
-    unfold iter, Iter_Kleisli, Basics.iter, MonadIter_itree, ITree.iter.
-    specialize (itree_eta (KTree.iter g a) ) as H. rewrite Hiter in H. simpl in H.
-    admit.
-  - admit.
+  intros. unfold spec_iter_arrow_rel in H. cbn in H. unfold _obsip in H. 
+  remember spin as t. rewrite Heqt. rewrite <- Heqt. assert (t ≈ spin). { rewrite Heqt. reflexivity. }
+  clear Heqt. gen_dep2 a t.
+  pcofix CIH. intros t Ht a Hwfa. 
+  pfold. punfold Hwfa; try apply not_wf_F_mono'.
+  inversion Hwfa. pclearbot.
+  specialize (unfold_iter_ktree g a) as Hiter. apply strong_to_weak_bisim in Hiter as Hiter'.
+  rewrite Hrel in Hiter'. setoid_rewrite bind_ret in Hiter'. 
+  apply observe_eutt_spin in  Ht as Ht0. basic_solve. red. rewrite H.
+  unfold iter, Iter_Kleisli, Basics.iter, MonadIter_itree, ITree.iter. unfold observe.
+  cbn. destruct (observe (g a) ) eqn : ?Heq; simpl; basic_solve.
+  - simpl. constructor; auto. right. apply CIH; auto.
+    specialize (itree_eta (g a) ) as Hga. rewrite Heq in Hga. rewrite Hga in Hrel. basic_solve. auto.
+  - exfalso. specialize (itree_eta (g a)) as Hga. rewrite Heq in Hga. rewrite Hga in Hrel. basic_solve.
+  - constructor. specialize (itree_eta (g a)) as Hga. rewrite Heq in Hga. rewrite Hga in Hiter. 
+
 Admitted.
+
+Lemma iter_morph_aux_l : forall (A B : Type) (g : A -> itree Void (A + B) ) (a : A) (p : itree Void B -> Prop)
+                                (Hp : resp_eutt _ _ p),  p (KTree.iter g a) -> _iter_fix (fun x => obs _ (g x) ) a p Hp.
+Proof.
+  intros. set (fun a1 a2 => a1 =[ fun x => obs _ (g x) ]=> a2) as rg.
+  destruct (classic (not_wf_from _ rg a) ).
+  - apply not_wf_iter_spin in H0 as Heutt. 
+    punfold H0; try apply not_wf_F_mono'. destruct H0. pclearbot. unfold rg in Hrel. unfold spec_iter_arrow_rel in Hrel.
+    cbn in Hrel. red in Hrel.
+    red. exists 1. simpl. red. eapply extern_div; eauto; auto. eapply Hp; eauto.
+  - specialize neg_wf_from_not_wf_from as Hn. specialize (Hn A rg). 
+    assert (wf_from A rg a).
+    { specialize (Hn a). destruct (classic (wf_from A rg a)); tauto. }
+    clear Hn H0.
+    induction H1.
+    + unfold rg in H0. destruct (eutt_reta_or_div _ (g a) ); basic_solve.
+      * rename a0 into a'. specialize (H0 a'). exfalso. apply H0. unfold spec_iter_arrow_rel.
+        cbn. red. symmetry. eauto.
+      * exists 1. cbn. red. symmetry in H1. eapply term_b; eauto.
+        eapply Hp; eauto. setoid_rewrite unfold_iter_ktree. rewrite H1. setoid_rewrite bind_ret. reflexivity.
+      * exists 1. cbn. red. eapply intern_div; eauto. apply div_spin_eutt in H1. eapply Hp; eauto.
+        setoid_rewrite unfold_iter_ktree. rewrite H1. apply spin_bind.
+    + destruct (eutt_reta_or_div _ (g a) ); basic_solve.
+      * rename a0 into a'. symmetry in H2. specialize (H1 a').
+        assert (rg a a').
+        { unfold rg. unfold spec_iter_arrow_rel. cbn. red. auto. }
+        assert (p (KTree.iter g a')).
+        { eapply Hp; eauto. setoid_rewrite  unfold_iter_ktree. rewrite H2.
+          setoid_rewrite <- unfold_iter_ktree. setoid_rewrite bind_ret. rewrite tau_eutt. reflexivity. }
+        specialize (H1 H3 H4). red in H1. basic_solve. exists (S n). cbn. red. eapply cont_a; eauto.
+      * exists 1. cbn. red. symmetry in H2. eapply term_b; eauto.
+        eapply Hp; eauto. setoid_rewrite unfold_iter_ktree. rewrite H2. setoid_rewrite bind_ret. reflexivity.
+      * exists 1. cbn. red. eapply intern_div; eauto. apply div_spin_eutt in H2. eapply Hp; eauto.
+        setoid_rewrite unfold_iter_ktree. rewrite H2. apply spin_bind.
+Qed.
+
+
 
 Lemma iter_morph : forall (A B : Type) (g : A -> itree Void (A + B) ) (a : A),
       obs _ (iter g a) ≈ iter_fix (fun x => obs _ (g x) ) a.
 Proof.
   constructor.
-  - intros. cbn in H. red in H. cbn.
-    (*need some notion of number of unfolds or extern div, that should be doable, *)
-    admit.
+  - intros. cbn in H. red in H. cbn. apply iter_morph_aux_l. auto.
   - intros. cbn. red. cbn in H. red in H. basic_solve. generalize dependent a. induction n; try contradiction.
-    intros. cbn in H.  red in H. inversion H; eauto. 
+    intros. cbn in H.  red in H. inversion H; eauto; clear H.
     + eapply Hp with (t1 := ret b); auto. setoid_rewrite unfold_iter_ktree.
       rewrite Hretb. setoid_rewrite bind_ret. reflexivity.
     + eapply Hp with (t1 := spin); auto. setoid_rewrite unfold_iter_ktree.
@@ -203,6 +257,55 @@ Proof.
     + apply Hp with (t1 := KTree.iter g a0); auto.
       setoid_rewrite unfold_iter_ktree with (a1 := a). rewrite Hreta. setoid_rewrite bind_ret.
       rewrite tau_eutt. reflexivity.
+Qed.
+
+
+Instance PureITreeIter :  Iter (Kleisli PureITreeSpec) sum := @iter_fix.
+
+Ltac unf_bindg := unfold bindpi, _bindpi.
+
+Ltac unf_bind H := unfold bindpi, _bindpi in H.
+
+Lemma itree_spec_iter_unfold_aux_l : forall A B (g : A -> PureITreeSpec (A + B) ) a n p Hp,
+    proj1_sig (iter_fix_n n g a) p Hp -> proj1_sig (cat g (case_ (iter_fix_n n g) (id_ B)) a) p Hp.
+Proof.
+  intros. generalize dependent a. induction n; try contradiction; intros.
+  cbn. unf_bindg. cbn in H. dest_dep g a. eapply Hfa; eauto. intros ?t ?Ht. inversion Ht; clear Ht; auto.
+  - left. exists (inr b). split; auto. symmetry. auto.
+  - punfold Hnwf; try apply not_wf_F_mono'. destruct Hnwf. unfold spec_iter_arrow_rel in Hrel. 
+    left. exists (inl a0). symmetry in Hreta. split; auto. cbn. pclearbot. dest_dep g a0.
+    eapply Hfa0; try apply Hrel. intros ?t ?Ht. simpl in *. eapply extern_div; eauto. auto.
+  -  specialize (IHn a0 Hrec) as IHn'. symmetry in Hreta. left. exists (inl a0). split; auto. cbn.
+     cbn in IHn'. unf_bind IHn'. dest_dep g a0. eapply Hfa0; try apply IHn'. intros ?t ?Ht. simpl in *.
+     basic_solve; eauto.
+     + cbn in H1. specialize (IHn a1 H1). eapply cont_a; eauto. symmetry. eauto.
+     + symmetry in H0. cbn in H1. red in H1. unfold id in *. eapply term_b; eauto. auto.
+Qed.
+
+Lemma itree_spec_iter_unfold_aux_r : forall A B (g : A -> PureITreeSpec (A + B) ) a n p Hp,
+    proj1_sig (cat g (case_ (iter_fix_n n g) (id_ B)) a) p Hp -> proj1_sig (iter_fix_n (S n) g a) p Hp.
+Proof.
+  intros. generalize dependent a. induction n; intros.
+  - cbn in H. unf_bind H. cbn. dest_dep g a. eapply Hfa; try apply H. intros ?t ?Ht.
+    simpl in *. basic_solve; eauto; try contradiction.
+    cbn in H1. red in H1. unfold id in *. symmetry in H0. eapply term_b; eauto. auto.
+  - cbn in H. unf_bind H. cbn. dest_dep g a. eapply Hfa; try apply H. intros ?t ?Ht.
+    simpl in *. basic_solve; eauto.
+    + symmetry in H0. eapply cont_a; try apply H0. auto.
+    + symmetry in H0. eapply term_b; try apply H0. auto.
+Qed.
+
+
+Instance PureITreeIterUnfold :  IterUnfold  (Kleisli PureITreeSpec) sum.
+Proof.
+  intros A B g.
+  constructor.
+  - specialize ( itree_spec_iter_unfold_aux_l A B g a) as H. cbn in H. cbn. intros. red in H0. basic_solve.
+    specialize (H n p Hp H0). unf_bindg. unf_bind H. dest_dep g a. eapply Hfa; try apply H. intros ?t ?Ht.
+    simpl in *. basic_solve; eauto. cbn in H2. left. exists (inl a0). split; auto. cbn.
+    exists n. auto.
+  - specialize  ( itree_spec_iter_unfold_aux_r A B g a) as H. cbn in H. cbn. intros. red.
+    unf_bind H0. dest_dep g a. 
 Admitted.
 
 
